src/Pipit.System.Exp.fst
@@ -1,24 +1,26 @@
 (* Translation to transition system *)
 module Pipit.System.Exp
 
-module C = Pipit.Context
+open Pipit.Prim.Table
+open Pipit.Exp.Base
+module Causal = Pipit.Exp.Causality
+
+module CR = Pipit.Context.Row
 
 open Pipit.System.Base
 open Pipit.System.Det
 
-open Pipit.Exp.Base
-module Causal = Pipit.Exp.Causality
 
 (* A system we get from translating an expression *)
-let xsystem (c: C.context) (state: Type) (value: Type) = system (C.row c) state value
+let xsystem (c: context) (state: Type) (value: Type) = system (row c) state value
 (* Same, but deterministic *)
-let xdsystem (c: C.context) (state: Type) (value: Type) = dsystem (C.row c) state value
+let xdsystem (c: context) (state: Type) (value: Type) = dsystem (row c) state value
 
 let xsystem_stepn
-  (#c: C.context)
+  (#c: context)
   (#state #value: Type)
   (t: xsystem c state value)
-  (streams: list (C.row c & value))
+  (streams: list (row c & value))
   (s': state): prop =
   system_stepn t streams s'
 
@@ -43,7 +45,7 @@ let rec dsystem_of_exp (e: exp 'c 'a { Causal.causal e }):
     Tot (xdsystem 'c (state_of_exp e) 'a) (decreases e) =
   match e with
   | XVal v -> dsystem_const v
-  | XBVar x -> dsystem_map (fun i -> C.row_index 'c i x) dsystem_input
+  | XBVar x -> dsystem_map (fun i -> CR.index 'c i x) dsystem_input
   | XVar x -> false_elim ()
   | XApp e1 e2 ->
     assert_norm (Causal.causal (XApp e1 e2) ==> (Causal.causal e1 && Causal.causal e2));
@@ -57,7 +59,7 @@ let rec dsystem_of_exp (e: exp 'c 'a { Causal.causal e }):
     dsystem_then (dsystem_of_exp e1) (dsystem_of_exp e2)
   | XMu _ e1 ->
     let t = dsystem_of_exp e1 in
-    dsystem_mu_causal #(C.row 'c) #('a & C.row 'c) (fun i v -> (v, i)) t
+    dsystem_mu_causal #(row 'c) #('a & row 'c) (fun i v -> (v, i)) t
   | XLet b e1 e2 ->
     dsystem_let (fun i v -> (v, i)) (dsystem_of_exp e1) (dsystem_of_exp e2)
   | XCheck name e1 e2 ->
@@ -72,7 +74,7 @@ let rec system_of_exp_rel (e: exp 'c 'a { Causal.causal e }):
   // else
     match e with
     | XVal v -> system_const v
-    | XBVar x -> system_map (fun i -> C.row_index 'c i x) system_input
+    | XBVar x -> system_map (fun i -> CR.index 'c i x) system_input
     | XVar x -> false_elim ()
     | XApp e1 e2 ->
       assert_norm (Causal.causal (XApp e1 e2) ==> (Causal.causal e1 && Causal.causal e2));
@@ -86,7 +88,7 @@ let rec system_of_exp_rel (e: exp 'c 'a { Causal.causal e }):
       system_then (system_of_exp_rel e1) (system_of_exp_rel e2)
     | XMu _ e1 ->
       let t = system_of_exp_rel e1 in
-      system_mu #(C.row 'c) #('a & C.row 'c) (fun i v -> (v, i)) t
+      system_mu #(row 'c) #('a & row 'c) (fun i v -> (v, i)) t
     | XLet b e1 e2 ->
       system_let (fun i v -> (v, i)) (system_of_exp_rel e1) (system_of_exp_rel e2)
     // | XContract assm guar body arg ->
